OrderBook.v
@@ -1,0 +1,78 @@
+Require Import
+        List.
+Require Import
+        Events
+        LibModel
+        Maps
+        Messages
+        States
+        Types.
+
+Module OrderBook.
+
+  Section SubmitOrder.
+
+    Definition submitOrder_spec (sender: address) (order: Order) : FSpec :=
+      {|
+        fspec_require :=
+          fun wst =>
+            (sender = order_owner order \/ sender = order_broker order) /\
+            H2O.find (ob_orders (wst_order_book_state wst))
+                     (get_order_hash order) = None
+        ;
+
+        fspec_trans :=
+          fun wst wst' retval =>
+            let hash := get_order_hash order in
+            let orders := ob_orders (wst_order_book_state wst) in
+            let orders' := H2O.upd orders hash order in
+            wst' = wst_update_order_book wst {| ob_orders := orders' |} /\
+            retval = RetBytes32 hash
+        ;
+
+        fspec_events :=
+          fun wst events =>
+            events = EvtOrderSubmitted sender (get_order_hash order) :: nil
+        ;
+      |}.
+
+  End SubmitOrder.
+
+  Section GetOrderData.
+
+    Definition getOrderData_spec (sender: address) (hash: bytes32) : FSpec :=
+      {|
+        fspec_require :=
+          fun wst => True;
+
+        fspec_trans :=
+          fun wst wst' retval =>
+            wst' = wst /\
+            retval = RetOrder (H2O.get (ob_orders (wst_order_book_state wst))
+                                       hash);
+
+        fspec_events :=
+          fun wst events => events = nil;
+      |}.
+
+  End GetOrderData.
+
+  Definition get_spec (msg: OrderBookMsg) : FSpec :=
+    match msg with
+    | msg_submitOrder sender order =>
+      submitOrder_spec sender order
+
+    | msg_getOrderData sender hash =>
+      getOrderData_spec sender hash
+    end.
+
+  Definition model
+             (wst: WorldState)
+             (msg: OrderBookMsg)
+             (wst': WorldState)
+             (retval: RetVal)
+             (events: list Event)
+    : Prop :=
+    fspec_sat (get_spec msg) wst wst' retval events.
+
+End OrderBook.
