Types.v
@@ -94,6 +94,35 @@ Record Order : Type :=
       order_walletSplitPercentage : uint16;
     }.
 
+Parameters get_order_hash: Order -> bytes32.
+
+Definition get_order_hash_preimg (order: Order) :=
+  (order_allOrNone order,
+   order_tokenBFeePercentage order,
+   order_tokenSFeePercentage order,
+   order_feePercentage order,
+   order_walletSplitPercentage order,
+   order_feeToken order,
+   order_tokenRecipient order,
+   order_wallet order,
+   order_orderInterceptor order,
+   order_broker order,
+   order_dualAuthAddr order,
+   order_tokenB order,
+   order_tokenS order,
+   order_owner order,
+   order_validUntil order,
+   order_validSince order,
+   order_feeAmount order,
+   order_amountB order,
+   order_amountS order).
+
+Axiom order_hash_dec:
+  forall (ord ord': Order),
+    let preimg := get_order_hash_preimg ord in
+    let preimg' := get_order_hash_preimg ord' in
+    (preimg = preimg' -> get_order_hash ord = get_order_hash ord') /\
+    (preimg <> preimg' -> get_order_hash ord <> get_order_hash ord').
 
 (** Ring *)
 Record Ring : Type :=
